<rdf:RDF xmlns="http://webtlab.it.uc3m.es/ns/hermes/driver#"
	xml:base="http://webtlab.it.uc3m.es/ns/hermes/driver"
	xmlns:rdf="http://www.w3.org/1999/02/22-rdf-syntax-ns#"
	xmlns:rdfs="http://www.w3.org/2000/01/rdf-schema#"
	xmlns:xsd="http://www.w3.org/2001/XMLschema#"
	xmlns:geo="http://www.w3.org/2003/01/geo/wgs84_pos#">


	<!--------------------------- CLASSES --------------------->
	
	<!------------  USERS / SENSORS -->
	
	<!--NOTE: Maybe we should talk about Sensors -attached to users-
	instead of Users directly. Cause in the future we may have general
	sensors, like AVM in buses, or things like that.--> 
	
	<rdfs:Class rdf:ID="User">
	</rdfs:Class>	
	
	<rdfs:Class rdf:ID="Driver">
		<rdfs:subClassOf rdf:resource="&hermes;User"/>
	</rdfs:Class>	
	
	<rdfs:Class rdf:ID="Pedestrian">
		<rdfs:subClassOf rdf:resource="&hermes;User"/>
	</rdfs:Class>
	
	<!------------  OBSERVATIONS -->
	
	<!--NOTE: Maybe we should talk about the properties that a particular 
	observation observes - and make a hierarchy of properties - instead of 
	making a hierarchy of observations -->
	
	<!-- I no longer see an observation as a type of 'Spatial Thing' -->
	<rdfs:Class rdf:ID="Observation">
		<rdfs:comment>
		An observation registered by a mobile or digital sensor from 
		a particular user in a moment of time.		
		</rdfs:comment>		
	</rdfs:Class>

	<!------------  OBSERVATIONS FROM SMART DRIVER-->
	
	<rdfs:Class rdf:ID="Driving">
		<rdfs:comment>
		An event registered by the sensor - smartphone - of a user 
		while driving a car. Two types of events: those appearing 
		when an unusual value occurs while driving, and those that 
		are automatically triggered when a driving section - a path in 
		the traveling - is completed.			
		</rdfs:comment>		
		<rdfs:subClassOf rdf:resource="&hermes;Observation"/>
	</rdfs:Class>
	
	<!--NOTE: The distinction of the two types of events does not make 
	sense in this representational level - it's an issue related to the 
	application, 'when' an observation is triggered-. 
	However, depending on the observation, we want to know the 
	distance of the path -if it is not an unexpected event -. -->
		
	<rdfs:Class rdf:ID="Speed">
		<rdfs:comment>
		An Observation related to the speed of the automobile.
		</rdfs:comment>		
		<rdfs:subClassOf rdf:resource="&hermes;Driving"/>
	</rdfs:Class>
	
	<rdfs:Class rdf:ID="Heart_Rate">
		<rdfs:comment>
		An Observation related to a driver pulse.
		</rdfs:comment>		
		<rdfs:subClassOf rdf:resource="&hermes;Driving"/>
	</rdfs:Class>
	
	<rdfs:Class rdf:ID="High_Heart_Rate">
		<rdfs:comment>
		An Observation related to a driver pulse when unexpected.
		It does not advise about the distance of the path.
		</rdfs:comment>		
		<rdfs:subClassOf rdf:resource="&hermes;Heart_Rate"/>
	</rdfs:Class>
	
	<rdfs:Class rdf:ID="Stopping">
		<rdfs:comment>
		An Observation related to the number of stops in a completed 
		path.		
		</rdfs:comment>		
		<rdfs:subClassOf rdf:resource="&hermes;Driving"/>
	</rdfs:Class>
	
	<rdfs:Class rdf:ID="Kinetics">
		<rdfs:comment>
		An Observation related to the driving agressivity, which
		depends on the frequency and intensity of possitive
		accelerations.
		</rdfs:comment>		
		<rdfs:subClassOf rdf:resource="&hermes;Driving"/>
	</rdfs:Class>
	
	<rdfs:Class rdf:ID="Acceleration">
		<rdfs:comment>
		An unexpected Observation related to driving acceleration.
		Either high acceleration or high deceleration can be observed.
		</rdfs:comment>		
		<rdfs:subClassOf rdf:resource="&hermes;Driving"/>
	</rdfs:Class>
	
	<!------------  OBSERVATIONS FROM FITBIT-->
	
	<rdfs:Class rdf:ID="Stepping">
		<rdfs:comment>
		An event registered by a user's Fitbit device	while walking -or running-.
		</rdfs:comment>		
		<rdfs:subClassOf rdf:resource="&hermes;Observation"/>
	</rdfs:Class>

	<rdfs:Class rdf:ID="Step_Set">
		<rdfs:comment>
		The set of steps given by a pedestrian and collected with the 
		Fitbit device.
		</rdfs:comment>				
	</rdfs:Class>


	<!------------------------ PROPERTIES -------------->
	
	<rdf:Property rdf:ID="has_user">
		<rdfs:comment>
			The owner of the the sensor that has detected the observation.
		</rdfs:comment>	
		<rdfs:domain rdf:resource="#Observation">
		<rdfs:range rdf:resource="#User"/>
	</rdf:Property>
	
	<rdf:Property rdf:ID="has_driver">
		<rdfs:comment>
			The owner of the the sensor that has detected the observation.
		</rdfs:comment>	
		<rdfs:subPropertyOf rdf:resource="&hermes;has_user"/>
		<rdfs:domain rdf:resource="#Driving">
		<rdfs:range rdf:resource="#Driver"/>
	</rdf:Property>
	
	<rdf:Property rdf:ID="has_pedestrian">
		<rdfs:comment>
			The owner of the the Fitbit device.
		</rdfs:comment>	
		<rdfs:subPropertyOf rdf:resource="&hermes;has_user"/>
		<rdfs:domain rdf:resource="#Stepping">
		<rdfs:range rdf:resource="#Pedestrian"/>
	</rdf:Property>
	
	<rdf:Property rdf:ID="uri">
		<rdfs:comment>
		This property can take the values N, NE, E, S, ES, SW, W or WN.
		</rdfs:comment>
		<rdfs:domain rdf:resource="#Observation">
		<rdf:range rdf:resource="&rdf;Literal">
	</rdf:Property>
	
	<rdf:Property rdf:ID="orientation">
		<rdfs:comment>
		This property can take the values N, NE, E, S, ES, SW, W or WN.
		</rdfs:comment>
		<rdfs:domain rdf:resource="#Driving">
		<rdf:range rdf:resource="&rdf;Literal">
	</rdf:Property>
	
	<rdf:Property rdf:ID="has_location">
		<rdfs:comment>
		The plot where this observation has been taken.
		Properties 'lat' and 'long' from geo points are in decimal 
		degrees, float points.
		</rdfs:comment>	
		<rdfs:domain rdf:resource="#Driving">
		<rdfs:range rdf:resource="&geo;SpatialThing"/>
	</rdf:Property>
	
	<rdf:Property rdf:ID="completed_distance">
		<rdfs:comment>
		The distance - in meters - of the section or path completed.
		</rdfs:comment>	
		<rdfs:domain rdf:resource="#SectionDriving">
		<rdfs:range rdf:resource="&xsd;float"/>
	</rdf:Property>
	
	<rdf:Property rdf:ID="speed_value">
		<rdfs:comment>
			The speed in km/h.
		</rdfs:comment>	
		<rdfs:domain rdf:resource="#Speed">
		<rdfs:range rdf:resource="&xsd;float"/>
	</rdf:Property>
	
	<rdf:Property rdf:ID="speed_type">
		<rdfs:comment>
			The kind of speed the Driving Observation have obtained.
			It can take the values: 
			- "deviation", for the standard deviation speed;
			- "average", for the average speed;
			- "low" or "high", for inefficient speed observed.
		</rdfs:comment>	
		<rdfs:domain rdf:resource="#Speed">
		<rdfs:range rdf:resource="&rdf;Literal"/>
	</rdf:Property>
	
	<rdf:Property rdf:ID="bpm">
		<rdfs:comment>
			The beats per minute of a driver, in b/min.
		</rdfs:comment>	
		<rdfs:domain rdf:resource="#Heart_Rate">
		<rdfs:range rdf:resource="&xsd;nonNegativeInteger"/>
	</rdf:Property>
	
	<rdf:Property rdf:ID="stops">
		<rdfs:comment>
			The number of stops in a completed path.
		</rdfs:comment>	
		<rdfs:domain rdf:resource="#Stopping">
		<rdfs:range rdf:resource="&xsd;nonNegativeInteger"/>
	</rdf:Property>	
	
	<rdf:Property rdf:ID="energy">
		<rdfs:comment>
			The positive kinetic energy value, in m/s2 -same as acceleration-.
		</rdfs:comment>	
		<rdfs:domain rdf:resource="#Kinetics">
		<rdfs:range rdf:resource="&xsd;float"/>
	</rdf:Property>
	
	<rdf:Property rdf:ID="acceleration">
		<rdfs:comment>
			The acceleration of an Observation, in m/s2.
			It refers to a deceleration when its value is less than 0.
		</rdfs:comment>	
		<rdfs:domain rdf:resource="#Acceleration">
		<rdfs:range rdf:resource="&xsd;float"/>
	</rdf:Property>
	
	<rdf:Property rdf:ID="on_date">
		<rdfs:comment>
		The day -yyyy/mm/dd- of the observed stepping.
		</rdfs:comment>	
		<rdfs:domain rdf:resource="#Stepping">
		<rdfs:range rdf:resource="&xsd;date"/>
	</rdf:Property>
	
	<rdf:Property rdf:ID="at_time">
		<rdfs:comment>
		The time -hh:mm:ss- of the observed stepping set.
		</rdfs:comment>	
		<rdfs:domain rdf:resource="#Step_Set">
		<rdfs:range rdf:resource="&xsd;time"/>
	</rdf:Property>
	
	<rdf:Property rdf:ID="stops">
		<rdfs:comment>
			The number of steps made by a Pedestrian for a particular date and time observed.
		</rdfs:comment>	
		<rdfs:domain rdf:resource="#Step_Set">
		<rdfs:range rdf:resource="&xsd;nonNegativeInteger"/>
	</rdf:Property>
	
	<rdf:Property rdf:ID="has_step_set">
		<rdfs:comment>
			The set of steps observed in a particular date and time.
		</rdfs:comment>			
		<rdfs:domain rdf:resource="#Stepping">
		<rdfs:range rdf:resource="#Step_Set"/>
	</rdf:Property>
	
</rdf:RDF>
